theories/common/StatePredicate.v
@@ -41,11 +41,11 @@ Section DEFINITIONS.
   Context `{!stateGS Σ}.
 
   Definition state_data (k : key) (v : Any.t) : stateF :=
-    discrete_fun_singleton k.1
+    discrete_fun_singleton (scope k)
       (reservation_map_data (A := stateV) (state_key_encode k) (Excl v)).
 
-  Definition state_token (scope : string) (E : coPset) : stateF :=
-    discrete_fun_singleton scope (reservation_map_token (A := stateV) E).
+  Definition state_token (scp : string) (E : coPset) : stateF :=
+    discrete_fun_singleton scp (reservation_map_token (A := stateV) E).
 
   Definition points_to_tgt (k : key) (v : Any.t) : iProp Σ :=
     own name_tgt (◯ state_data k v).
@@ -53,17 +53,17 @@ Section DEFINITIONS.
   Definition points_to_src (k : key) (v : Any.t) : iProp Σ :=
     own name_src (◯ state_data k v).
 
-  Definition uninit_tgt_scope (scope : string) (E : coPset) : iProp Σ :=
-    own name_tgt (◯ state_token scope E).
+  Definition uninit_tgt_scope (scp : string) (E : coPset) : iProp Σ :=
+    own name_tgt (◯ state_token scp E).
 
-  Definition uninit_src_scope (scope : string) (E : coPset) : iProp Σ :=
-    own name_src (◯ state_token scope E).
+  Definition uninit_src_scope (scp : string) (E : coPset) : iProp Σ :=
+    own name_src (◯ state_token scp E).
 
   Definition uninit_tgt (k : key) : iProp Σ :=
-    uninit_tgt_scope k.1 {[ state_key_encode k ]}.
+    uninit_tgt_scope (scope k) {[ state_key_encode k ]}.
 
   Definition uninit_src (k : key) : iProp Σ :=
-    uninit_src_scope k.1 {[ state_key_encode k ]}.
+    uninit_src_scope (scope k) {[ state_key_encode k ]}.
 
   Definition state_cell_tgt (k : key) (ov : option Any.t) : iProp Σ :=
     match ov with
@@ -82,34 +82,34 @@ Section DEFINITIONS.
 
   Definition state_slice (S : gset string)
       (m : gmap key (option Any.t)) : gmap key Any.t :=
-    filter (fun kv : key * Any.t => kv.1.1 ∈ S) (live_state m).
+    filter (fun kv : key * Any.t => scope kv.1 ∈ S) (live_state m).
 
-  Definition state_entries (scope : string)
+  Definition state_entries (scp : string)
       (m : gmap key (option Any.t)) : gmap key Any.t :=
-    filter (fun kv : key * Any.t => kv.1.1 = scope) (live_state m).
+    filter (fun kv : key * Any.t => scope kv.1 = scp) (live_state m).
 
-  Definition state_values (scope : string)
+  Definition state_values (scp : string)
       (m : gmap key (option Any.t)) : gmap positive stateV :=
-    kmap state_key_encode (Excl <$> state_entries scope m).
+    kmap state_key_encode (Excl <$> state_entries scp m).
 
-  Definition state_fields (scope : string)
+  Definition state_fields (scp : string)
       (m : gmap key (option Any.t)) : gset positive :=
-    dom (state_values scope m).
+    dom (state_values scp m).
 
-  Definition state_uninit_set (scope : string)
+  Definition state_uninit_set (scp : string)
       (m : gmap key (option Any.t)) : coPset :=
-    ⊤ ∖ gset_to_coPset (state_fields scope m).
+    ⊤ ∖ gset_to_coPset (state_fields scp m).
 
   Definition state_present (m : gmap key (option Any.t)) : stateF :=
-    fun scope =>
-      ReservationMap (state_values scope m)
-        (CoPset (state_uninit_set scope m)).
+    fun scp =>
+      ReservationMap (state_values scp m)
+        (CoPset (state_uninit_set scp m)).
 
   Definition state_absent (S : gset string)
       (m : gmap key (option Any.t)) : stateF :=
-    fun scope =>
-      if decide (scope ∈ S)
-      then reservation_map_token (A := stateV) (state_uninit_set scope m)
+    fun scp =>
+      if decide (scp ∈ S)
+      then reservation_map_token (A := stateV) (state_uninit_set scp m)
       else ε.
 
   Definition state_points (S : gset string)
@@ -118,13 +118,13 @@ Section DEFINITIONS.
 
   Definition state_fragment (S : gset string)
       (m : gmap key (option Any.t)) : stateF :=
-    fun scope =>
-      if decide (scope ∈ S) then state_present m scope else ε.
+    fun scp =>
+      if decide (scp ∈ S) then state_present m scp else ε.
 
   Definition state_fragment_rest (S : gset string)
       (m : gmap key (option Any.t)) : stateF :=
-    fun scope =>
-      if decide (scope ∈ S) then ε else state_present m scope.
+    fun scp =>
+      if decide (scp ∈ S) then ε else state_present m scp.
 
   Definition SI_tgt (m : gmap key (option Any.t)) : iProp Σ :=
     own name_tgt (● state_present m).
@@ -160,12 +160,12 @@ Section BASIC_LEMMAS.
 
   Context `{!stateGS Σ}.
 
-  #[local] Instance stateF_lookup_op_homomorphism scope :
+  #[local] Instance stateF_lookup_op_homomorphism scp :
       MonoidHomomorphism op op (≡)
-        (fun f : stateF => f scope).
+        (fun f : stateF => f scp).
   Proof.
     split; [split|]; try apply _.
-    - intros n f g EQ. exact (EQ scope).
+    - intros n f g EQ. exact (EQ scp).
     - intros f g. by rewrite discrete_fun_lookup_op.
     - done.
   Qed.
@@ -179,36 +179,36 @@ Section BASIC_LEMMAS.
 
   Lemma state_slice_lookup S m k :
     state_slice S m !! k =
-      if decide (k.1 ∈ S) then mjoin (m !! k) else None.
+      if decide (scope k ∈ S) then mjoin (m !! k) else None.
   Proof.
     rewrite /state_slice map_lookup_filter live_state_lookup.
-    destruct (decide (k.1 ∈ S)) as [IN|NIN].
+    destruct (decide (scope k ∈ S)) as [IN|NIN].
     - destruct (mjoin (m !! k)); simpl; by repeat case_guard.
     - destruct (mjoin (m !! k)); simpl; by repeat case_guard.
   Qed.
 
-  Lemma state_slice_lookup_in S m k (IN : k.1 ∈ S) :
+  Lemma state_slice_lookup_in S m k (IN : scope k ∈ S) :
     state_slice S m !! k = mjoin (m !! k).
   Proof. rewrite state_slice_lookup. by case_decide. Qed.
 
-  Lemma state_slice_lookup_notin S m k (NIN : k.1 ∉ S) :
+  Lemma state_slice_lookup_notin S m k (NIN : scope k ∉ S) :
     state_slice S m !! k = None.
   Proof. rewrite state_slice_lookup. by case_decide. Qed.
 
-  Lemma state_data_lookup k v scope :
-    state_data k v scope =
-      if decide (k.1 = scope)
+  Lemma state_data_lookup k v scp :
+    state_data k v scp =
+      if decide (scope k = scp)
       then reservation_map_data (A := stateV)
         (state_key_encode k) (Excl v)
       else ε.
   Proof.
     rewrite /state_data.
-    destruct (decide (k.1 = scope)) as [EQ|NEQ].
-    - subst scope. by rewrite discrete_fun_lookup_singleton.
+    destruct (decide (scope k = scp)) as [EQ|NEQ].
+    - subst scp. by rewrite discrete_fun_lookup_singleton.
     - by rewrite discrete_fun_lookup_singleton_ne.
   Qed.
 
-  Lemma state_slice_insert S m k v (IN : k.1 ∈ S) :
+  Lemma state_slice_insert S m k v (IN : scope k ∈ S) :
     state_slice S (<[k := Some v]> m) = <[k := v]> (state_slice S m).
   Proof.
     rewrite /state_slice /live_state (omap_insert_Some id m k (Some v) v) //.
@@ -222,7 +222,8 @@ Section BASIC_LEMMAS.
     rewrite map_filter_delete. done.
   Qed.
 
-  Lemma state_slice_set_state_cell_eq S m1 m2 k ov (IN : k.1 ∈ S)
+  Lemma state_slice_set_state_cell_eq S m1 m2 k ov
+      (IN : scope k ∈ S)
       (EQ : state_slice S m1 = state_slice S m2) :
     state_slice S (set_state_cell k ov m1) =
       state_slice S (set_state_cell k ov m2).
@@ -237,24 +238,24 @@ Section BASIC_LEMMAS.
     state_slice (S1 ∪ S2) m = state_slice S1 m ∪ state_slice S2 m.
   Proof.
     rewrite /state_slice -map_filter_or -map_filter_ext.
-    intros [scope field] v LOOK. simpl. set_solver.
+    intros [scp field] v LOOK. simpl. set_solver.
   Qed.
 
   Lemma state_slice_disjoint S1 S2 m (DISJ : S1 ## S2) :
     state_slice S1 m ##ₘ state_slice S2 m.
   Proof.
     apply elem_of_disjoint in DISJ.
-    rewrite map_disjoint_spec. intros [scope field] x y LOOK1 LOOK2.
+    rewrite map_disjoint_spec. intros [scp field] x y LOOK1 LOOK2.
     rewrite /state_slice in LOOK1, LOOK2.
     apply map_lookup_filter_Some in LOOK1.
     apply map_lookup_filter_Some in LOOK2.
     destruct LOOK1 as [_ IN1]. destruct LOOK2 as [_ IN2].
     simpl in IN1, IN2.
-    exact (DISJ scope IN1 IN2).
+    exact (DISJ scp IN1 IN2).
   Qed.
 
   Lemma state_values_lookup m k :
-    state_values k.1 m !! state_key_encode k =
+    state_values (scope k) m !! state_key_encode k =
       Excl <$> live_state m !! k.
   Proof.
     rewrite /state_values lookup_kmap lookup_fmap
@@ -262,15 +263,15 @@ Section BASIC_LEMMAS.
     destruct (live_state m !! k); simpl; by repeat case_guard.
   Qed.
 
-  Lemma state_values_insert m k v scope :
-    state_values scope (<[k := Some v]> m) =
-      if decide (k.1 = scope)
-      then <[state_key_encode k := Excl v]> (state_values scope m)
-      else state_values scope m.
+  Lemma state_values_insert m k v scp :
+    state_values scp (<[k := Some v]> m) =
+      if decide (scope k = scp)
+      then <[state_key_encode k := Excl v]> (state_values scp m)
+      else state_values scp m.
   Proof.
     rewrite /state_values /state_entries /live_state
       (omap_insert_Some id m k (Some v) v) //.
-    destruct (decide (k.1 = scope)) as [EQ|NEQ].
+    destruct (decide (scope k = scp)) as [EQ|NEQ].
     - rewrite map_filter_insert_True; last done.
       rewrite fmap_insert kmap_insert. done.
     - rewrite map_filter_insert_False; last done.
@@ -280,7 +281,7 @@ Section BASIC_LEMMAS.
   Qed.
 
   Lemma elem_of_state_fields m k :
-    state_key_encode k ∈ state_fields k.1 m ↔
+    state_key_encode k ∈ state_fields (scope k) m ↔
       is_Some (live_state m !! k).
   Proof.
     rewrite /state_fields elem_of_dom state_values_lookup.
@@ -288,7 +289,7 @@ Section BASIC_LEMMAS.
   Qed.
 
   Lemma elem_of_state_uninit_set m k :
-    state_key_encode k ∈ state_uninit_set k.1 m ↔
+    state_key_encode k ∈ state_uninit_set (scope k) m ↔
       live_state m !! k = None.
   Proof.
     rewrite /state_uninit_set elem_of_difference elem_of_top
@@ -296,19 +297,19 @@ Section BASIC_LEMMAS.
     rewrite eq_None_not_Some. tauto.
   Qed.
 
-  Lemma state_fields_slice_ext S m1 m2 scope
-      (IN : scope ∈ S) (EQ : state_slice S m1 = state_slice S m2) :
-    state_fields scope m1 = state_fields scope m2.
+  Lemma state_fields_slice_ext S m1 m2 scp
+      (IN : scp ∈ S) (EQ : state_slice S m1 = state_slice S m2) :
+    state_fields scp m1 = state_fields scp m2.
   Proof.
     assert (FILTER : ∀ m,
-        state_entries scope m =
-          filter (fun kv : key * Any.t => kv.1.1 = scope)
+        state_entries scp m =
+          filter (fun kv : key * Any.t => scope kv.1 = scp)
             (state_slice S m)).
     { intros m. rewrite /state_entries /state_slice.
       symmetry. apply map_filter_filter_l.
       intros [key_scope field] v LOOK EQSCOPE. simpl in *.
       by subst key_scope. }
-    assert (ENTRIES : state_entries scope m1 = state_entries scope m2).
+    assert (ENTRIES : state_entries scp m1 = state_entries scp m2).
     { rewrite !FILTER EQ. done. }
     by rewrite /state_fields /state_values ENTRIES.
   Qed.
@@ -317,35 +318,36 @@ Section BASIC_LEMMAS.
       (EQ : state_slice S m1 = state_slice S m2) :
     state_absent S m1 ≡ state_absent S m2.
   Proof.
-    intros scope. rewrite /state_absent /state_uninit_set.
-    destruct (decide (scope ∈ S)) as [IN|NIN]; last done.
-    by rewrite (state_fields_slice_ext S m1 m2 scope IN EQ).
+    intros scp. rewrite /state_absent /state_uninit_set.
+    destruct (decide (scp ∈ S)) as [IN|NIN]; last done.
+    by rewrite (state_fields_slice_ext S m1 m2 scp IN EQ).
   Qed.
 
-  Lemma state_fields_insert m k v scope :
-    state_fields scope (<[k := Some v]> m) =
-      if decide (k.1 = scope)
-      then {[state_key_encode k]} ∪ state_fields scope m
-      else state_fields scope m.
+  Lemma state_fields_insert m k v scp :
+    state_fields scp (<[k := Some v]> m) =
+      if decide (scope k = scp)
+      then {[state_key_encode k]} ∪ state_fields scp m
+      else state_fields scp m.
   Proof.
     rewrite /state_fields state_values_insert.
-    destruct (decide (k.1 = scope)); first by rewrite dom_insert_L.
+    destruct (decide (scope k = scp)); first by rewrite dom_insert_L.
     done.
   Qed.
 
   Lemma state_absent_insert_new S m k v
-      (IN : k.1 ∈ S) (NONE : live_state m !! k = None) :
+      (IN : scope k ∈ S) (NONE : live_state m !! k = None) :
     state_absent S m ≡
-      state_token k.1 {[state_key_encode k]} ⋅
+      state_token (scope k) {[state_key_encode k]} ⋅
         state_absent S (<[k := Some v]> m).
   Proof.
-    intros scope.
+    intros scp.
     rewrite discrete_fun_lookup_op /state_absent /state_token.
-    destruct (decide (scope ∈ S)) as [INS|NINS].
-    - destruct (decide (k.1 = scope)) as [EQ|NEQ].
-      + subst scope. rewrite discrete_fun_lookup_singleton.
-        assert (ABS : state_uninit_set k.1 (<[k := Some v]> m) =
-            state_uninit_set k.1 m ∖ {[state_key_encode k]}).
+    destruct (decide (scp ∈ S)) as [INS|NINS].
+    - destruct (decide (scope k = scp)) as [EQ|NEQ].
+      + subst scp. rewrite discrete_fun_lookup_singleton.
+        assert (ABS : state_uninit_set (scope k)
+            (<[k := Some v]> m) =
+            state_uninit_set (scope k) m ∖ {[state_key_encode k]}).
         { apply set_eq. intros i.
           rewrite /state_uninit_set state_fields_insert.
           case_decide; last contradiction.
@@ -357,8 +359,8 @@ Section BASIC_LEMMAS.
         rewrite elem_of_state_uninit_set. exact NONE.
       + rewrite discrete_fun_lookup_singleton_ne // left_id.
         rewrite /state_uninit_set state_fields_insert. case_decide; done.
-    - destruct (decide (k.1 = scope)) as [EQ|NEQ].
-      + subst scope. exfalso. set_solver.
+    - destruct (decide (scope k = scp)) as [EQ|NEQ].
+      + subst scp. exfalso. set_solver.
       + rewrite discrete_fun_lookup_singleton_ne // left_id. done.
   Qed.
 
@@ -366,30 +368,30 @@ Section BASIC_LEMMAS.
     state_absent (S1 ∪ S2) m ≡
       state_absent S1 m ⋅ state_absent S2 m.
   Proof.
-    apply elem_of_disjoint in DISJ. intros scope.
+    apply elem_of_disjoint in DISJ. intros scp.
     rewrite discrete_fun_lookup_op /state_absent.
-    destruct (decide (scope ∈ S1)) as [IN1|NIN1];
-      destruct (decide (scope ∈ S2)) as [IN2|NIN2].
-    - exfalso. exact (DISJ scope IN1 IN2).
-    - destruct (decide (scope ∈ S1 ∪ S2)) as [IN|NIN].
+    destruct (decide (scp ∈ S1)) as [IN1|NIN1];
+      destruct (decide (scp ∈ S2)) as [IN2|NIN2].
+    - exfalso. exact (DISJ scp IN1 IN2).
+    - destruct (decide (scp ∈ S1 ∪ S2)) as [IN|NIN].
       + by rewrite right_id.
       + exfalso. apply NIN. set_solver.
-    - destruct (decide (scope ∈ S1 ∪ S2)) as [IN|NIN].
+    - destruct (decide (scp ∈ S1 ∪ S2)) as [IN|NIN].
       + by rewrite left_id.
       + exfalso. apply NIN. set_solver.
-    - destruct (decide (scope ∈ S1 ∪ S2)) as [IN|NIN].
+    - destruct (decide (scp ∈ S1 ∪ S2)) as [IN|NIN].
       + exfalso. set_solver.
       + by rewrite left_id.
   Qed.
 
   Lemma state_fields_insert_existing m k v old
-      (LOOK : live_state m !! k = Some old) scope :
-    state_fields scope (<[k := Some v]> m) = state_fields scope m.
+      (LOOK : live_state m !! k = Some old) scp :
+    state_fields scp (<[k := Some v]> m) = state_fields scp m.
   Proof.
     rewrite state_fields_insert.
-    destruct (decide (k.1 = scope)) as [EQ|NEQ]; last done.
-    subst scope.
-    assert (IN : state_key_encode k ∈ state_fields k.1 m).
+    destruct (decide (scope k = scp)) as [EQ|NEQ]; last done.
+    subst scp.
+    assert (IN : state_key_encode k ∈ state_fields (scope k) m).
     { rewrite elem_of_state_fields. eauto. }
     apply set_eq. intros i. rewrite elem_of_union elem_of_singleton.
     split.
@@ -401,36 +403,36 @@ Section BASIC_LEMMAS.
       (LOOK : live_state m !! k = Some old) :
     state_absent S (<[k := Some v]> m) ≡ state_absent S m.
   Proof.
-    intros scope.
+    intros scp.
     rewrite /state_absent /state_uninit_set.
-    by rewrite (state_fields_insert_existing m k v old LOOK scope).
+    by rewrite (state_fields_insert_existing m k v old LOOK scp).
   Qed.
 
   Lemma state_absent_insert_value S m k v1 v2 :
     state_absent S (<[k := Some v1]> m) ≡
       state_absent S (<[k := Some v2]> m).
   Proof.
-    intros scope. rewrite /state_absent /state_uninit_set.
+    intros scp. rewrite /state_absent /state_uninit_set.
     by rewrite !state_fields_insert.
   Qed.
 
   Lemma state_present_valid m : ✓ state_present m.
   Proof.
-    intros scope. rewrite /state_present reservation_map_valid_eq /=.
+    intros scp. rewrite /state_present reservation_map_valid_eq /=.
     split.
     - intros i.
-      destruct (state_values scope m !! i) as [[x|]|] eqn:LOOK.
+      destruct (state_values scp m !! i) as [[x|]|] eqn:LOOK.
       + exact I.
       + have BAD := LOOK.
         apply lookup_kmap_Some in BAD as (k & -> & BAD).
         2: apply state_key_encode_inj.
         rewrite lookup_fmap in BAD.
-        destruct (state_entries scope m !! k) as [y|] eqn:ENTRY;
+        destruct (state_entries scp m !! k) as [y|] eqn:ENTRY;
           [change (Some (Excl y) = Some ExclInvalid) in BAD
           |change (None = Some (@ExclInvalid Any.t)) in BAD];
           discriminate BAD.
       + exact I.
-    - intros i. destruct (state_values scope m !! i) as [x|] eqn:LOOK;
+    - intros i. destruct (state_values scp m !! i) as [x|] eqn:LOOK;
         last by left.
       right. rewrite /state_uninit_set elem_of_difference elem_of_top
         elem_of_gset_to_coPset. intros [_ NIN]. apply NIN.
@@ -457,11 +459,12 @@ Section BASIC_LEMMAS.
       + rewrite left_id. done.
   Qed.
 
-  Lemma state_slice_scope S m scope :
-    filter (fun kv : key * Any.t => kv.1.1 = scope) (state_slice S m) =
-      if decide (scope ∈ S) then state_entries scope m else ∅.
+  Lemma state_slice_scope S m scp :
+    filter (fun kv : key * Any.t => scope kv.1 = scp)
+      (state_slice S m) =
+      if decide (scp ∈ S) then state_entries scp m else ∅.
   Proof.
-    destruct (decide (scope ∈ S)) as [IN|NIN].
+    destruct (decide (scp ∈ S)) as [IN|NIN].
     - rewrite /state_slice /state_entries.
       apply map_filter_filter_l.
       intros [key_scope field] v LOOK EQSCOPE. simpl in *.
@@ -473,21 +476,21 @@ Section BASIC_LEMMAS.
       subst key_scope. contradiction.
   Qed.
 
-  Lemma state_points_filter (sm : gmap key Any.t) scope :
+  Lemma state_points_filter (sm : gmap key Any.t) scp :
     ([^op map] k ↦ v ∈ sm,
-      if decide (k.1 = scope)
+      if decide (scope k = scp)
       then reservation_map_data (A := stateV)
         (state_key_encode k) (Excl v)
       else ε) ≡
     ([^op map] k ↦ v ∈
-      filter (fun kv : key * Any.t => kv.1.1 = scope) sm,
+      filter (fun kv : key * Any.t => scope kv.1 = scp) sm,
       reservation_map_data (A := stateV)
         (state_key_encode k) (Excl v)).
   Proof.
     induction sm as [|k v sm NONE IH] using map_ind.
     - rewrite map_filter_empty !big_opM_empty. done.
     - rewrite big_opM_insert //.
-      destruct (decide (k.1 = scope)) as [EQ|NEQ].
+      destruct (decide (scope k = scp)) as [EQ|NEQ].
       + rewrite map_filter_insert_True; last done.
         rewrite big_opM_insert; last by rewrite map_lookup_filter NONE.
         rewrite IH. done.
@@ -497,30 +500,31 @@ Section BASIC_LEMMAS.
         rewrite left_id IH. done.
   Qed.
 
-  Lemma state_points_lookup S m scope :
-    state_points S m scope ≡
-      if decide (scope ∈ S)
-      then (ReservationMap (state_values scope m) ε :
+  Lemma state_points_lookup S m scp :
+    state_points S m scp ≡
+      if decide (scp ∈ S)
+      then (ReservationMap (state_values scp m) ε :
         reservation_map stateV)
       else ε.
   Proof.
     rewrite /state_points
-      (big_opM_commute (fun f : stateF => f scope)
+      (big_opM_commute (fun f : stateF => f scp)
         (fun k v => state_data k v) (state_slice S m)).
     transitivity ([^op map] k ↦ v ∈ state_slice S m,
-      if decide (k.1 = scope)
+      if decide (scope k = scp)
       then reservation_map_data (A := stateV)
         (state_key_encode k) (Excl v)
       else ε).
     { apply big_opM_proper. intros k v LOOK.
       rewrite state_data_lookup. done. }
     transitivity ([^op map] k ↦ v ∈
-      filter (fun kv : key * Any.t => kv.1.1 = scope) (state_slice S m),
+      filter (fun kv : key * Any.t => scope kv.1 = scp)
+        (state_slice S m),
       reservation_map_data (A := stateV)
         (state_key_encode k) (Excl v)).
     { apply state_points_filter. }
     rewrite state_slice_scope.
-    destruct (decide (scope ∈ S)) as [IN|NIN].
+    destruct (decide (scp ∈ S)) as [IN|NIN].
     - rewrite reservation_map_points /state_values. done.
     - rewrite big_opM_empty. done.
   Qed.
@@ -528,9 +532,9 @@ Section BASIC_LEMMAS.
   Lemma state_fragment_points S m :
     state_fragment S m ≡ state_points S m ⋅ state_absent S m.
   Proof.
-    intros scope. rewrite discrete_fun_lookup_op state_points_lookup
+    intros scp. rewrite discrete_fun_lookup_op state_points_lookup
       /state_fragment /state_absent /state_present.
-    destruct (decide (scope ∈ S)); last by rewrite left_id.
+    destruct (decide (scp ∈ S)); last by rewrite left_id.
     rewrite /op /cmra_op /=. split; simpl.
     - by rewrite right_id.
     - by rewrite left_id.
@@ -539,9 +543,9 @@ Section BASIC_LEMMAS.
   Lemma state_fragment_included S m :
     state_fragment S m ≼ state_present m.
   Proof.
-    exists (state_fragment_rest S m). intros scope.
+    exists (state_fragment_rest S m). intros scp.
     rewrite discrete_fun_lookup_op /state_fragment /state_fragment_rest.
-    destruct (decide (scope ∈ S)); by rewrite ?left_id ?right_id.
+    destruct (decide (scp ∈ S)); by rewrite ?left_id ?right_id.
   Qed.
 
   Local Lemma state_points_sep γ S m :
@@ -639,35 +643,36 @@ Section BASIC_LEMMAS.
     (state_present m, state_data k v) ~l~>
       (state_present (<[k := Some vn]> m), state_data k vn).
   Proof.
-    apply discrete_fun_local_update. intros scope.
+    apply discrete_fun_local_update. intros scp.
     rewrite /state_present /state_data.
-    destruct (decide (k.1 = scope)) as [EQ|NEQ].
-    - subst scope. rewrite !discrete_fun_lookup_singleton state_values_insert.
+    destruct (decide (scope k = scp)) as [EQ|NEQ].
+    - subst scp. rewrite !discrete_fun_lookup_singleton state_values_insert.
       case_decide; try contradiction.
       rewrite /state_uninit_set
-        (state_fields_insert_existing m k vn v LOOK k.1).
+        (state_fields_insert_existing m k vn v LOOK (scope k)).
       apply reservation_map_replace_local_update.
       by rewrite state_values_lookup LOOK.
     - rewrite !discrete_fun_lookup_singleton_ne //.
       rewrite state_values_insert. case_decide; try contradiction.
       rewrite /state_uninit_set
-        (state_fields_insert_existing m k vn v LOOK scope).
+        (state_fields_insert_existing m k vn v LOOK scp).
       reflexivity.
   Qed.
 
   Lemma state_present_insert_local m k v
       (NONE : live_state m !! k = None) :
     (state_present m,
-      state_token k.1 {[state_key_encode k]}) ~l~>
+      state_token (scope k) {[state_key_encode k]}) ~l~>
       (state_present (<[k := Some v]> m), state_data k v).
   Proof.
-    apply discrete_fun_local_update. intros scope.
+    apply discrete_fun_local_update. intros scp.
     rewrite /state_present /state_token /state_data.
-    destruct (decide (k.1 = scope)) as [EQ|NEQ].
-    - subst scope. rewrite !discrete_fun_lookup_singleton state_values_insert.
+    destruct (decide (scope k = scp)) as [EQ|NEQ].
+    - subst scp. rewrite !discrete_fun_lookup_singleton state_values_insert.
       case_decide; try contradiction.
-      assert (ABS : state_uninit_set k.1 (<[k := Some v]> m) =
-          state_uninit_set k.1 m ∖ {[state_key_encode k]}).
+      assert (ABS : state_uninit_set (scope k)
+          (<[k := Some v]> m) =
+          state_uninit_set (scope k) m ∖ {[state_key_encode k]}).
       { apply set_eq. intros i.
         rewrite /state_uninit_set state_fields_insert.
         case_decide; try contradiction.
@@ -687,12 +692,13 @@ Section BASIC_LEMMAS.
     live_state m !! k = Some v.
   Proof.
     apply auth_both_valid_discrete in VALID as [INCL _].
-    have INCL_SCOPE := discrete_fun_included_spec_1 _ _ k.1 INCL.
+    have INCL_SCOPE :=
+      discrete_fun_included_spec_1 _ _ (scope k) INCL.
     rewrite /state_data discrete_fun_lookup_singleton /state_present
       reservation_map_included in INCL_SCOPE.
     destruct INCL_SCOPE as [DATA _].
-    assert (VALUES_VALID : ✓ state_values k.1 m).
-    { have VALID := state_present_valid m k.1.
+    assert (VALUES_VALID : ✓ state_values (scope k) m).
+    { have VALID := state_present_valid m (scope k).
       rewrite reservation_map_valid_eq /= in VALID.
       destruct VALID as [VALUES_VALID _]. exact VALUES_VALID. }
     rewrite /reservation_map_data /=
@@ -705,11 +711,12 @@ Section BASIC_LEMMAS.
 
   Lemma state_present_uninit_lookup m k
       (VALID : ✓ (● state_present m ⋅
-        ◯ state_token k.1 {[state_key_encode k]})) :
+        ◯ state_token (scope k) {[state_key_encode k]})) :
     live_state m !! k = None.
   Proof.
     apply auth_both_valid_discrete in VALID as [INCL _].
-    have INCL_SCOPE := discrete_fun_included_spec_1 _ _ k.1 INCL.
+    have INCL_SCOPE :=
+      discrete_fun_included_spec_1 _ _ (scope k) INCL.
     rewrite /state_token discrete_fun_lookup_singleton /state_present
       reservation_map_included in INCL_SCOPE.
     destruct INCL_SCOPE as [_ TOKEN].
@@ -739,10 +746,10 @@ Section BASIC_LEMMAS.
     iPureIntro. destruct (m !! k) as [[w|]|]; inversion LIVE. done.
   Qed.
 
-  Lemma uninit_tgt_scope_split scope E i (IN : i ∈ E) :
-    uninit_tgt_scope scope E ⊣⊢
-      uninit_tgt_scope scope {[i]} ∗
-      uninit_tgt_scope scope (E ∖ {[i]}).
+  Lemma uninit_tgt_scope_split scp E i (IN : i ∈ E) :
+    uninit_tgt_scope scp E ⊣⊢
+      uninit_tgt_scope scp {[i]} ∗
+      uninit_tgt_scope scp (E ∖ {[i]}).
   Proof.
     rewrite /uninit_tgt_scope /state_token.
     rewrite -own_op -auth_frag_op.
@@ -751,10 +758,10 @@ Section BASIC_LEMMAS.
     set_solver.
   Qed.
 
-  Lemma uninit_src_scope_split scope E i (IN : i ∈ E) :
-    uninit_src_scope scope E ⊣⊢
-      uninit_src_scope scope {[i]} ∗
-      uninit_src_scope scope (E ∖ {[i]}).
+  Lemma uninit_src_scope_split scp E i (IN : i ∈ E) :
+    uninit_src_scope scp E ⊣⊢
+      uninit_src_scope scp {[i]} ∗
+      uninit_src_scope scp (E ∖ {[i]}).
   Proof.
     rewrite /uninit_src_scope /state_token.
     rewrite -own_op -auth_frag_op.
@@ -888,7 +895,7 @@ Section INIT_ACCESS.
   Context {Σ : GRA}.
 
   Lemma state_init_tgt_acc `{STATE : !stateGS Σ} S m k
-      (SCOPE : k.1 ∈ S) :
+      (SCOPE : scope k ∈ S) :
     state_init_tgt S m STATE ⊢
       ∃ ov, ⌜ov = mjoin (m !! k)⌝ ∗ state_cell_tgt k ov ∗
         (∀ ov', ⌜state_cell_transition ov ov'⌝ -∗
@@ -940,7 +947,7 @@ Section INIT_ACCESS.
   Qed.
 
   Lemma state_init_src_acc `{STATE : !stateGS Σ} S m k
-      (SCOPE : k.1 ∈ S) :
+      (SCOPE : scope k ∈ S) :
     state_init_src S m STATE ⊢
       ∃ ov, ⌜ov = mjoin (m !! k)⌝ ∗ state_cell_src k ov ∗
         (∀ ov', ⌜state_cell_transition ov ov'⌝ -∗
